Alpha.v
@@ -1,0 +1,1151 @@
+
+(** Alternative definitions of substs and alpha for named formulas *)
+
+Require Import RelationClasses Arith Omega Defs Proofs Nam.
+Import ListNotations.
+Local Open Scope bool_scope.
+Local Open Scope lazy_bool_scope.
+Local Open Scope eqb_scope.
+
+Arguments Vars.union _ _ : simpl nomatch.
+
+(** Alternative definition of substitution,
+    closer to the initial document,
+    but needs induction over height, due to double recursive call *)
+
+Fixpoint form_height f :=
+  match f with
+  | True | False | Pred _ _ => 0
+  | Not f => S (form_height f)
+  | Op _ f1 f2 => S (Nat.max (form_height f1) (form_height f2))
+  | Quant _ _ f => S (form_height f)
+  end.
+
+Fixpoint form_substH h x t f :=
+ match h with
+ | 0 => True
+ | S h =>
+   match f with
+   | True | False => f
+   | Pred p args => Pred p (List.map (term_subst x t) args)
+   | Not f => Not (form_substH h x t f)
+   | Op o f f' => Op o (form_substH h x t f) (form_substH h x t f')
+   | Quant q v f' =>
+     if x =? v then f
+     else
+       let out_vars := term_vars t in
+       if negb (Vars.mem v out_vars) then
+         Quant q v (form_substH h x t f')
+       else
+         (* variable capture : we change v into a fresh variable first *)
+         let z := fresh_var (vars_unions [allvars f; out_vars; Vars.singleton x])
+         in
+         Quant q z (form_substH h x t (form_substH h v (Var z) f'))
+   end
+ end.
+
+Definition form_subst x t f :=
+ form_substH (S (form_height f)) x t f.
+
+(** Basic results about [form_subst] *)
+
+Ltac simpl_height :=
+ match goal with
+ | H : S _ < S _ |- _ =>
+   apply Nat.succ_lt_mono in H; simpl_height
+ | H : Nat.max _ _ < _ |- _ =>
+   apply Nat.max_lub_lt_iff in H; destruct H; simpl_height
+ | _ => idtac
+ end.
+
+Lemma form_substH_height v t f h :
+  form_height f < h ->
+  form_height (form_substH h v t f) = form_height f.
+Proof.
+ revert v t f.
+ induction h.
+ - inversion 1.
+ - intros v t [ ] LT; simpl in *; simpl_height; auto.
+   case eqb; auto.
+   case negb; simpl; auto.
+   repeat rewrite IHh; auto.
+Qed.
+
+Lemma form_subst_height v t f :
+  form_height (form_subst v t f) = form_height f.
+Proof.
+ apply form_substH_height; auto with *.
+Qed.
+
+Lemma form_substH_indep v t f h h' :
+  form_height f < h -> form_height f < h' ->
+  form_substH h v t f = form_substH h' v t f.
+Proof.
+ revert h' v t f.
+ induction h; [inversion 1|]; destruct h';[inversion 2|].
+ destruct f; cbn -[fresh_var]; intros; simpl_height; f_equal; auto.
+ case eqbspec; intros; auto.
+ destruct negb eqn:E; f_equal; auto.
+ rewrite (IHh h' v0) by auto.
+ apply IHh; rewrite form_substH_height; auto.
+Qed.
+
+Lemma form_substH_subst v t f h :
+  form_height f < h ->
+  form_substH h v t f = form_subst v t f.
+Proof.
+ intros. apply form_substH_indep; auto with *.
+Qed.
+
+Lemma form_subst_eqn x t f :
+ form_subst x t f =
+ match f with
+ | True => True
+ | False => False
+ | Pred p l => Pred p (List.map (term_subst x t) l)
+ | Not f => Not (form_subst x t f)
+ | Op o f f' => Op o (form_subst x t f) (form_subst x t f')
+ | Quant q v f' =>
+    if x =? v then f
+    else
+      let out_vars := term_vars t in
+      if negb (Vars.mem v out_vars) then
+        Quant q v (form_subst x t f')
+      else
+        let z := fresh_var (vars_unions [allvars f; out_vars; Vars.singleton x])
+      in
+        Quant q z (form_subst x t (form_subst v (Var z) f'))
+ end.
+Proof.
+ destruct f; try reflexivity.
+ - unfold form_subst.
+   set (h1 := S (form_height f1)).
+   set (h2 := S (form_height f2)).
+   set (h := form_height _).
+   assert (LT1 : form_height f1 < h1) by (cbn; auto with * ).
+   assert (LT2 : form_height f2 < h2) by (cbn; auto with * ).
+   assert (LT1' : form_height f1 < h) by (cbn; auto with * ).
+   assert (LT2' : form_height f2 < h) by (cbn; auto with * ).
+   clearbody h h1 h2.
+   cbn. f_equal; apply form_substH_indep; auto.
+ - unfold form_subst. rewrite form_substH_height; auto with *.
+Qed.
+
+(** Before studying more this full substitution,
+    we consider a partial version, sufficient to define
+    alpha-equivalence *)
+
+Fixpoint partialsubst x t f :=
+  match f with
+  | True | False => f
+  | Pred p args => Pred p (List.map (term_subst x t) args)
+  | Not f => Not (partialsubst x t f)
+  | Op o f f' => Op o (partialsubst x t f) (partialsubst x t f')
+  | Quant q v f' =>
+    Quant q v
+     (if (x=?v) || Vars.mem v (term_vars t) then f'
+      else partialsubst x t f')
+  end.
+
+(** Places where [form_subst] and [partialsubst] will agree *)
+
+Fixpoint IsSimple v t f :=
+  match f with
+  | True | False | Pred _ _ => Logic.True
+  | Not f => IsSimple v t f
+  | Op _ f f' => IsSimple v t f /\ IsSimple v t f'
+  | Quant _ x f => v = x \/ (~Vars.In x (term_vars t)
+                             /\ IsSimple v t f)
+  end.
+
+(** Inductive description of these "simple" substitutions *)
+
+Inductive SimpleSubst (v:variable)(t:term)
+ : formula -> formula -> Prop :=
+| SubTr : SimpleSubst v t True True
+| SubFa : SimpleSubst v t False False
+| SubPred p l :
+  SimpleSubst v t (Pred p l) (Pred p (List.map (term_subst v t) l))
+| SubNot f f' :
+    SimpleSubst v t f f' ->
+    SimpleSubst v t (Not f) (Not f')
+| SubOp o f1 f2 f1' f2' :
+    SimpleSubst v t f1 f1' ->
+    SimpleSubst v t f2 f2' ->
+    SimpleSubst v t (Op o f1 f2) (Op o f1' f2')
+| SubQu1 q f : SimpleSubst v t (Quant q v f) (Quant q v f)
+| SubQu2 q f f' x : x<>v -> ~Vars.In x (term_vars t) ->
+    SimpleSubst v t f f' ->
+    SimpleSubst v t (Quant q x f) (Quant q x f').
+
+Hint Constructors SimpleSubst.
+
+Lemma SimpleSubst_fun v t f f1 f2 :
+ SimpleSubst v t f f1 -> SimpleSubst v t f f2 -> f1 = f2.
+Proof.
+ intros H1. revert f2.
+ induction H1; inversion 1; subst; f_equal; auto; easy.
+Qed.
+
+Lemma vars_mem_false x vs : ~Vars.In x vs -> Vars.mem x vs = false.
+Proof.
+ rewrite <- Vars.mem_spec. now case Vars.mem.
+Qed.
+
+Lemma SimpleSubst_substH x t f h :
+  form_height f < h ->
+  IsSimple x t f ->
+  SimpleSubst x t f (form_substH h x t f).
+Proof.
+ revert f.
+ induction h.
+ - inversion 1.
+ - destruct f; cbn -[fresh_var];
+   intros Hf IS; simpl_height; auto.
+   + intuition.
+   + case eqbspec.
+     * intros ->; auto.
+     * intros NE.
+       destruct IS as [->|(NI,SI)]; [easy|].
+       rewrite vars_mem_false; cbn; auto.
+Qed.
+
+Lemma SimpleSubst_subst x t f :
+  IsSimple x t f ->
+  SimpleSubst x t f (form_subst x t f).
+Proof.
+ apply SimpleSubst_substH. auto with *.
+Qed.
+
+Lemma SimpleSubst_IsSimple x t f f' :
+  SimpleSubst x t f f' -> IsSimple x t f.
+Proof.
+ induction 1; cbn; auto.
+Qed.
+
+Lemma SimpleSubst_partialsubst x t f :
+  IsSimple x t f ->
+  SimpleSubst x t f (partialsubst x t f).
+Proof.
+ induction f; cbn; auto.
+ - intuition.
+ - case eqbspec; cbn; intros Hxv IS; subst; auto.
+   destruct IS as [->|(NI,IS)]; [easy|].
+   rewrite vars_mem_false; auto.
+Qed.
+
+Lemma partialsubst_subst x t f :
+  IsSimple x t f -> partialsubst x t f = form_subst x t f.
+Proof.
+ intros IS. apply (SimpleSubst_fun x t f).
+ now apply SimpleSubst_partialsubst.
+ now apply SimpleSubst_subst.
+Qed.
+
+Lemma SimpleSubst_carac x t f f' :
+  SimpleSubst x t f f' <->
+   partialsubst x t f = f' /\ IsSimple x t f.
+Proof.
+  assert (H := SimpleSubst_partialsubst x t f).
+  split.
+  - intros H'.
+    assert (IS := SimpleSubst_IsSimple x t f f' H').
+    split; auto.
+    apply SimpleSubst_fun with x t f; auto.
+  - intros (<-,IS); auto.
+Qed.
+
+
+(** A sufficient condition for simplicity: *)
+
+Lemma noninter_issimple x t f :
+  Vars.Empty (Vars.inter (allvars f) (term_vars t)) -> IsSimple x t f.
+Proof.
+ induction f; cbn in *; auto.
+ intros E; split; (apply IHf1 || apply IHf2); varsdec.
+ intros E.
+ case (eqbspec v x).
+ - now left.
+ - intros NE. right; split; try apply IHf; varsdec.
+Qed.
+
+
+Lemma term_subst_notin x u t :
+ ~Vars.In x (term_vars t) ->
+ term_subst x u t = t.
+Proof.
+ induction t as [v|f a IH] using term_ind'; cbn.
+ - case eqbspec; auto. varsdec.
+ - intros NI. f_equal. apply map_id_iff.
+   intros t Ht. apply IH; auto. rewrite vars_unionmap_in in NI.
+   contradict NI. now exists t.
+Qed.
+
+
+Lemma partialsubst_notin x t f :
+ ~Vars.In x (freevars f) ->
+ partialsubst x t f = f.
+Proof.
+ induction f; cbn; intros NI; f_equal; auto with set.
+ - apply map_id_iff. intros a Ha. apply term_subst_notin.
+   rewrite vars_unionmap_in in NI. contradict NI. now exists a.
+ - case eqbspec; cbn; auto.
+   intros NE. case Vars.mem; f_equal; auto with set.
+Qed.
+
+Lemma partialsubst_height x t f :
+ form_height (partialsubst x t f) = form_height f.
+Proof.
+ induction f; cbn; auto. f_equal.
+ destruct orb; auto.
+Qed.
+
+Lemma partialsubst_height_lt x t f h :
+ form_height f < h -> form_height (partialsubst x t f) < h.
+Proof.
+ now rewrite partialsubst_height.
+Qed.
+
+Hint Resolve partialsubst_height_lt.
+
+Lemma freevars_allvars f : Vars.Subset (freevars f) (allvars f).
+Proof.
+ induction f; cbn; auto with set.
+Qed.
+
+Lemma term_subst_subst x u y v t :
+ x<>y -> ~Vars.In x (term_vars v) ->
+  term_subst y v (term_subst x u t) =
+  term_subst x (term_subst y v u) (term_subst y v t).
+Proof.
+ intros NE NI.
+ induction t using term_ind'; cbn.
+ - case eqbspec; [intros ->|intros NE'].
+   + change Vars.elt with variable in *.
+     rewrite <- eqb_neq in NE. rewrite NE. cbn.
+     now rewrite eqb_refl.
+   + case eqbspec; [intros ->|intros NE''].
+     * cbn. rewrite eqb_refl.
+       symmetry. now apply term_subst_notin.
+     * cbn. rewrite <-eqb_neq in NE',NE''. now rewrite NE', NE''.
+ - f_equal.
+   rewrite !map_map.
+   apply map_ext_in.
+   auto.
+Qed.
+
+Lemma SimpleSubst_SimpleSubst x u y v A B C B' C' :
+ x<>y -> ~Vars.In x (term_vars v) ->
+ SimpleSubst x u A B -> SimpleSubst y v B C ->
+ SimpleSubst y v A B' -> SimpleSubst x (term_subst y v u) B' C' ->
+ C = C'.
+Proof.
+ intros NE NI.
+ revert B C B' C'.
+ induction A.
+ - do 4 inversion 1; now subst.
+ - do 4 inversion 1; now subst.
+ - do 4 inversion 1. subst.
+   rewrite !map_map. f_equal.
+   apply map_ext. intros.
+   apply term_subst_subst; auto.
+ - do 4 inversion 1. subst. f_equal. eauto.
+ - do 4 inversion 1. subst. f_equal; eauto.
+ - do 4 inversion 1; subst; try easy; auto.
+   + f_equal. eapply SimpleSubst_fun; eauto.
+   + f_equal. rewrite term_subst_notin in * by auto.
+     eapply SimpleSubst_fun; eauto.
+   + f_equal. eauto.
+Qed.
+
+Lemma IsSimple_partialsubst x t v t' f :
+  IsSimple x t f ->
+  IsSimple x t (partialsubst v t' f).
+Proof.
+ induction f; cbn; try (intuition; fail).
+ intros [->|(NI,IS)]; [now left| right].
+ split; auto.
+ destruct orb; auto.
+Qed.
+
+Lemma partialsubst_partialsubst x u y v f :
+ x<>y -> ~Vars.In x (term_vars v) ->
+ IsSimple x u f ->
+ IsSimple y v f ->
+ IsSimple x (term_subst y v u) (partialsubst y v f) ->
+ partialsubst y v (partialsubst x u f) =
+ partialsubst x (term_subst y v u) (partialsubst y v f).
+Proof.
+ intros NE NI IS1 IS2 IS3.
+ assert (IS2' := IsSimple_partialsubst y v x u f IS2).
+ apply SimpleSubst_partialsubst in IS1.
+ apply SimpleSubst_partialsubst in IS2.
+ apply SimpleSubst_partialsubst in IS2'.
+ apply SimpleSubst_partialsubst in IS3.
+ eapply SimpleSubst_SimpleSubst. eauto. eauto.
+ apply IS1. apply IS2'. apply IS2. apply IS3.
+Qed.
+
+(* TODO : direct proof on partialsubst ??
+          are all hypotheses mandatory ??
+Lemma form_partialsubst_partialsubst x u y v f :
+ x<>y -> ~Vars.In x (term_vars v) ->
+ IsSimple x u f ->
+(* IsSimple y v (partialsubst x u f) -> *)
+ IsSimple y v f ->
+(* IsSimple x (term_subst y v u) (partialsubst y v f) -> *)
+ partialsubst y v (partialsubst x u f) =
+ partialsubst x (term_subst y v u) (partialsubst y v f).
+Proof.
+ intros NE NI.
+ induction f; cbn; intros IS1 IS2; auto.
+ - f_equal. rewrite !map_map.
+   apply map_ext. intros.
+   apply term_subst_subst; auto.
+ - f_equal; auto.
+ - f_equal; intuition.
+ - repeat (case eqbspec; cbn; auto); intros; subst; try easy.
+   + clear IS1. destruct IS2 as [->|(_,IS)]; [easy|].
+     rewrite <- Vars.mem_spec in NI.
+     apply not_true_is_false in NI. rewrite NI; auto.
+     cbn. now rewrite eqb_refl.
+   + clear IS2. destruct IS1 as [->|(NI',IS)]; [easy|].
+     rewrite <- Vars.mem_spec in NI'.
+     apply not_true_is_false in NI'. rewrite NI'; auto.
+     cbn. rewrite eqb_refl. cbn.
+     destruct (Vars.mem v0 (term_vars (term_subst v0 v u))) eqn:E';
+     f_equal; auto.
+     * admit.
+     * rewrite term_subst_notin; auto.
+       rewrite <- Vars.mem_spec. now rewrite NI'.
+   + destruct IS1 as [->|(NI1,IS1)]; [easy|].
+     destruct IS2 as [->|(NI2,IS2)]; [easy|].
+     rewrite <- Vars.mem_spec in NI1,NI2.
+     apply not_true_is_false in NI1.
+     apply not_true_is_false in NI2. rewrite NI1,NI2; auto.
+     cbn.
+     repeat (case eqbspec; cbn; auto); intros; subst; try easy.
+     rewrite NI2.
+     destruct (Vars.mem v0 (term_vars (term_subst y v u))) eqn:E;
+     f_equal; auto.
+     rewrite IHf; auto.
+     apply partialsubst_notin.
+*)
+
+(* TODO: useless ??
+Lemma IsSimple_Quant_carac x t q v f :
+ IsSimple x t (Quant q v f) ->
+  x=v /\ partialsubst x t (Quant q v f) = Quant q v f
+ \/
+  x<>v /\ ~Vars.In v (term_vars t) /\ IsSimple x t f /\
+  partialsubst x t (Quant q v f) = Quant q v (partialsubst x t f).
+Proof.
+ simpl.
+ case eqbspec.
+ - left; cbn; auto.
+ - intros NE [EQ|(NI,IS)]; [easy|].
+   right; cbn; repeat split; auto.
+   now rewrite vars_mem_false.
+Qed.
+*)
+
+(** Free variables after subst *)
+
+Lemma term_vars_subst x u t :
+ Vars.Subset (term_vars (term_subst x u t))
+             (Vars.union (Vars.remove x (term_vars t)) (term_vars u)).
+Proof.
+ induction t using term_ind'; cbn.
+ - case eqbspec; cbn; auto with set.
+ - intros v. rewrite vars_unionmap_in.
+   intros (a & IN & IN'). rewrite in_map_iff in IN'.
+   destruct IN' as (b & <- & IN').
+   apply H in IN; trivial.
+   revert IN.
+   VarsF.set_iff. rewrite vars_unionmap_in in *.
+   intros [(U,V)|W].
+   + left. split; auto. now exists b.
+   + now right.
+Qed.
+
+Lemma term_vars_subst_in x u t :
+ Vars.In x (term_vars t) ->
+ Vars.Equal (term_vars (term_subst x u t))
+            (Vars.union (Vars.remove x (term_vars t)) (term_vars u)).
+Proof.
+ revert t.
+ fix IH 1; destruct t; cbn.
+ - case eqbspec; cbn; auto with set.
+ - revert l.
+   fix IH' 1; destruct l; cbn.
+   + varsdec.
+   + destruct (VarsP.In_dec x (term_vars t)) as [E|E];
+     destruct (VarsP.In_dec x (vars_unionmap term_vars l)) as [E'|E'].
+     * intros _.
+       fold (term_subst x u t). rewrite (IH t E).
+       rewrite (IH' l E'). varsdec.
+     * intros _.
+       assert (E'' : map (term_substs [(x, u)]) l = l).
+       { apply map_id_iff. intros a Ha.
+         apply term_subst_notin. contradict E'.
+         rewrite vars_unionmap_in. now exists a. }
+       change Vars.elt with variable in *.
+       rewrite E''.
+       fold (term_subst x u t). rewrite (IH t E).
+       varsdec.
+     * intros _.
+       fold (term_subst x u t).
+       rewrite (term_subst_notin x u t) by trivial.
+       rewrite (IH' l E'). varsdec.
+     * VarsF.set_iff. tauto.
+Qed.
+
+Lemma term_vars_subst_in' x u t :
+ Vars.In x (term_vars t) ->
+ Vars.Subset (term_vars u) (term_vars (term_subst x u t)).
+Proof.
+ induction t using term_ind'; cbn.
+ - case eqbspec; cbn; auto with set.
+ - intros IN v Hv. rewrite vars_unionmap_in in *.
+   destruct IN as (a & Ha & IN).
+   exists (term_subst x u a); split; auto using in_map.
+   now apply (H a IN Ha).
+Qed.
+
+Lemma allvars_partialsubst x t f :
+ Vars.Subset (allvars (partialsubst x t f))
+             (Vars.union (allvars f) (term_vars t)).
+Proof.
+ induction f; cbn; try varsdec.
+ - generalize (term_vars_subst x t (Fun "" l)). cbn. varsdec.
+ - destruct orb; cbn; varsdec.
+Qed.
+
+Lemma allvars_partialsubst_2 x t f :
+ IsSimple x t f ->
+ Vars.In x (freevars f) ->
+ Vars.Subset (term_vars t) (allvars (partialsubst x t f)).
+Proof.
+ induction f; cbn; intros IS; try varsdec.
+ - apply (term_vars_subst_in' x t (Fun "" l)).
+ - auto.
+ - VarsF.set_iff. destruct IS as (IS1,IS2).
+   intros [IN|IN].
+   rewrite (IHf1 IS1 IN). varsdec.
+   rewrite (IHf2 IS2 IN). varsdec.
+ - case eqbspec; cbn. varsdec.
+   VarsF.set_iff. intros NE (IN,_).
+   destruct IS as [->|(NI,IS)]; [easy|].
+   specialize (IHf IS IN).
+   rewrite vars_mem_false by trivial. cbn. varsdec.
+Qed.
+
+Lemma freevars_partialsubst_in x t f :
+ IsSimple x t f ->
+ Vars.In x (freevars f) ->
+ Vars.Equal (freevars (partialsubst x t f))
+            (Vars.union (Vars.remove x (freevars f)) (term_vars t)).
+Proof.
+ induction f; cbn; intros IS IN.
+ - varsdec.
+ - varsdec.
+ - apply (term_vars_subst_in x t (Fun "" l)); auto.
+ - auto.
+ - destruct IS as (IS1,IS2).
+   rewrite Vars.union_spec in IN.
+   destruct (VarsP.In_dec x (freevars f1)) as [IN1|IN1];
+    destruct (VarsP.In_dec x (freevars f2)) as [IN2|IN2];
+    try rewrite (IHf1 IS1 IN1); try rewrite (IHf2 IS2 IN2);
+    try rewrite (partialsubst_notin x t f2) by trivial;
+    try rewrite (partialsubst_notin x t f1) by trivial;
+    varsdec.
+ - case eqbspec; cbn. varsdec.
+   intros. destruct IS as [->|(NI,IS)]; [easy|].
+   assert (IN' : Vars.In x (freevars f)) by varsdec.
+   rewrite vars_mem_false by trivial.
+   rewrite (IHf IS IN').
+   varsdec.
+Qed.
+
+
+Lemma freevars_partialsubst_subset x t f :
+ IsSimple x t f ->
+ Vars.Subset (freevars (partialsubst x t f))
+             (Vars.union (Vars.remove x (freevars f)) (term_vars t)).
+Proof.
+ induction f; cbn; intros IS.
+ - varsdec.
+ - varsdec.
+ - apply (term_vars_subst x t (Fun "" l)).
+ - auto.
+ - destruct IS as (IS1,IS2).
+   specialize (IHf1 IS1). specialize (IHf2 IS2). varsdec.
+ - case eqbspec; cbn. varsdec.
+   intros. destruct IS as [->|(NI,IS)]; [easy|].
+   specialize (IHf IS).
+   rewrite vars_mem_false by trivial.
+   cbn. varsdec.
+Qed.
+
+Lemma freevars_partialsubst_subset' x t f :
+  IsSimple x t f ->
+  Vars.Subset (freevars f)
+              (Vars.add x (freevars (partialsubst x t f))).
+Proof.
+ intros NE.
+ destruct (VarsP.In_dec x (freevars f)).
+ - rewrite freevars_partialsubst_in; auto with set.
+ - rewrite partialsubst_notin; auto with set.
+Qed.
+
+(** ALPHA EQUIVALENCE *)
+
+
+Inductive AlphaEq : formula -> formula -> Prop :=
+| AEqTr : AlphaEq True True
+| AEqFa : AlphaEq False False
+| AEqPred p l : AlphaEq (Pred p l) (Pred p l)
+| AEqNot f f' : AlphaEq f f' -> AlphaEq (Not f) (Not f')
+| AEqOp o f1 f2 f1' f2' :
+  AlphaEq f1 f1' -> AlphaEq f2 f2' ->
+  AlphaEq (Op o f1 f2) (Op o f1' f2')
+| AEqQu q v v' f f' z :
+  ~Vars.In z (Vars.union (allvars f) (allvars f')) ->
+  AlphaEq (partialsubst v (Var z) f) (partialsubst v' (Var z) f') ->
+  AlphaEq (Quant q v f) (Quant q v' f').
+Hint Constructors AlphaEq.
+
+Lemma get_fresh_var vars : exists z, ~Vars.In z vars.
+Proof.
+ exists (fresh_var vars). apply fresh_var_ok.
+Qed.
+
+Ltac simpl_fresh vars H :=
+ unfold vars in H; cbn in H;
+ rewrite ?Vars.add_spec, ?Vars.union_spec in H;
+ repeat (apply Decidable.not_or in H; destruct H as (?,H));
+ clear vars H.
+
+Lemma form_height_ind (P : formula -> Prop) :
+ (forall h, (forall f, form_height f < h -> P f) ->
+            (forall f, form_height f < S h -> P f)) ->
+ forall f, P f.
+Proof.
+ intros IH f.
+ set (h := S (form_height f)).
+ assert (LT : form_height f < h) by (cbn; auto with * ).
+ clearbody h. revert f LT.
+ induction h as [|h IHh]; [inversion 1|eauto].
+Qed.
+
+Lemma AEq_refl f :
+ AlphaEq f f.
+Proof.
+ induction f as [h IH f LT] using form_height_ind.
+ destruct f; cbn in *; simpl_height; auto.
+ destruct (get_fresh_var (allvars f)) as (z,Hz).
+ apply AEqQu with (z:=z); auto with set.
+Qed.
+
+Lemma AEq_sym f f' :
+ AlphaEq f f' -> AlphaEq f' f.
+Proof.
+ revert f'.
+ induction f as [h IH f LT] using form_height_ind.
+ destruct f, f'; cbn in *; simpl_height;
+   try (inversion_clear 1; auto).
+ apply AEqQu with (z:=z); auto with set.
+Qed.
+
+Lemma string_compare_eq (a b:variable) :
+  match (a ?= b)%string with
+  | Eq => true
+  | _ => false
+  end = (a =? b).
+Proof.
+ reflexivity.
+Qed.
+
+Lemma AEq_freevars f f' :
+  AlphaEq f f' -> Vars.Equal (freevars f) (freevars f').
+Proof.
+ induction 1; cbn; auto with set.
+ revert IHAlphaEq.
+ destruct (VarsP.In_dec v (freevars f)) as [E|E];
+  destruct (VarsP.In_dec v' (freevars f')) as [E'|E'];
+  try (rewrite (partialsubst_notin v (Var z) f E));
+  try (rewrite (partialsubst_notin v' (Var z) f' E'));
+  repeat (rewrite freevars_partialsubst_in by
+             ( auto; apply noninter_issimple; cbn; varsdec));
+  cbn;
+  rewrite <-!freevars_allvars in H.
+ - (* varsdec take ages ?! *)
+   intros EQ x. split.
+   { intros Hx. specialize (EQ x). varsdec. }
+   { intros Hx. specialize (EQ x). varsdec. }
+ - intros EQ x. split.
+   { intros Hx. specialize (EQ x). varsdec. }
+   { intros Hx. specialize (EQ x). varsdec. }
+ - intros EQ x. split.
+   { intros Hx. specialize (EQ x). varsdec. }
+   { intros Hx. specialize (EQ x). varsdec. }
+ - varsdec.
+Qed.
+
+Lemma term_subst_rename x x' z z' t t':
+  ~Vars.In z (Vars.union (term_vars t) (term_vars t')) ->
+  ~Vars.In z' (Vars.union (term_vars t) (term_vars t')) ->
+  term_subst x (Var z) t = term_subst x' (Var z) t'  ->
+  term_subst x (Var z') t = term_subst x' (Var z') t'.
+Proof.
+ revert t t'.
+ fix IH 1. destruct t, t'; intros Hz Hz'; cbn in *; try easy.
+ - do 2 case eqbspec; intros H H'; subst; intros [=]; varsdec.
+ - case eqbspec; intros _ [=].
+ - case eqbspec; intros _ [=].
+ - intros [= <- E]. f_equal. clear f.
+   revert l l0 Hz Hz' E.
+   fix IH' 1. destruct l, l0; intros Hz Hz'; cbn in *; try easy.
+   intros [= E E']. f_equal.
+   + apply IH; auto. varsdec. varsdec.
+   + apply IH'; auto. varsdec. varsdec.
+Qed.
+
+(** TODO : clean-up the next one (?) *)
+
+Lemma AEq_rename_aux f f' x x' v z z0 :
+  ~Vars.In z (Vars.union (Vars.add x (allvars f))
+                         (Vars.add v (allvars f'))) ->
+  ~Vars.In z0 (Vars.union (allvars f)
+                         (allvars (partialsubst x' (Var z) f'))) ->
+  AlphaEq (partialsubst x (Var z0) f)
+          (partialsubst v (Var z0) (partialsubst x' (Var z) f')) ->
+  ~Vars.In x' (freevars f').
+Proof.
+ intros Hz Hz0 EQ IN.
+ assert (IsSimple x (Var z0) f)
+   by (apply noninter_issimple; cbn; varsdec).
+ assert (IsSimple x' (Var z) f')
+   by (apply noninter_issimple; cbn; varsdec).
+ assert (z0 <> z).
+ { contradict Hz0. subst z0.
+   VarsF.set_iff. right.
+   rewrite <- freevars_allvars.
+   rewrite freevars_partialsubst_in; auto. cbn. varsdec. }
+ assert (NI : ~Vars.In z (freevars (partialsubst x (Var z0) f))).
+ { rewrite freevars_partialsubst_subset; auto. cbn.
+   rewrite freevars_allvars. varsdec. }
+ apply AEq_freevars in EQ.
+ rewrite EQ in NI.
+ contradict NI.
+ destruct (VarsP.In_dec v (freevars (partialsubst x' (Var z) f'))) as [E'|E'].
+ - rewrite freevars_partialsubst_in; auto.
+   cbn.
+   VarsF.set_iff.
+   rewrite freevars_partialsubst_in; auto. cbn. varsdec.
+   apply noninter_issimple. cbn. varsdec.
+ - rewrite partialsubst_notin by auto.
+   rewrite freevars_partialsubst_in; auto. cbn. varsdec.
+Qed.
+
+(* The crucial lemma, utterly technical for something so obvious *)
+
+Lemma AEq_rename_any x x' f f' z z' :
+  ~Vars.In z (Vars.union (allvars f) (allvars f')) ->
+  ~Vars.In z' (Vars.union (allvars f) (allvars f')) ->
+   AlphaEq (partialsubst x (Var z) f) (partialsubst x' (Var z) f') ->
+   AlphaEq (partialsubst x (Var z') f) (partialsubst x' (Var z') f').
+Proof.
+ revert f' x x' z z'.
+ induction f as [h IH f LT] using form_height_ind.
+ destruct f, f'; intros x x' z z' Hz Hz'; cbn in *; simpl_height;
+  try (inversion 1; auto; fail).
+ - inversion 1; subst.
+   assert (E : map (term_subst x (Var z')) l =
+                map (term_subst x' (Var z')) l0).
+   { injection (term_subst_rename x x' z z' (Fun "" l) (Fun "" l0)).
+     auto. varsdec. varsdec. cbn; f_equal; auto. }
+   now rewrite E.
+ - inversion 1; eauto.
+ - inversion 1; subst; constructor; eapply IH; eauto; varsdec.
+ - repeat match goal with |- context [(?a ?= ?b)%string] =>
+    fold (a =? b)%string; destruct (string_eqb_spec a b);
+     [exfalso; varsdec|]
+   end.
+   repeat (case eqbspec; cbn).
+   + trivial.
+   + intros NE <-. inversion_clear 1.
+     assert (~Vars.In x' (freevars f')).
+     { eapply AEq_rename_aux; eauto. }
+     rewrite !(partialsubst_notin x') in * by trivial.
+     apply AEqQu with z0; auto with set.
+   + intros <- NE. inversion_clear 1.
+     assert (~Vars.In x (freevars f)).
+     { apply AEq_sym in H1.
+       eapply AEq_rename_aux; eauto. varsdec. varsdec. }
+     rewrite !(partialsubst_notin x) in * by trivial.
+     apply AEqQu with z0; auto with set.
+   + intros NE NE'. inversion_clear 1.
+
+     (* Let's pick a suitably fresh variable z1 *)
+
+     set (vars :=
+            Vars.add x (Vars.add x' (Vars.add z (Vars.add z'
+             (vars_unions
+               [ allvars (partialsubst x (Var z) f);
+                allvars (partialsubst x' (Var z) f');
+                allvars f; allvars f']))))).
+     destruct (get_fresh_var vars) as (z1,Hz1).
+     simpl_fresh vars Hz1.
+
+     (* Let's use z1 instead of z0 in the main hyp *)
+
+     apply IH with (z':=z1) in H1; [ | auto | auto | varsdec].
+     clear H0 z0.
+
+     (* Let's use z1 in the conclusion. *)
+
+     apply AEqQu with z1; auto.
+     rewrite !allvars_partialsubst. cbn. varsdec.
+
+     revert H1.
+
+     (* We now need to swap the substitutions to
+        change z' with z thanks to the IH. *)
+
+     rewrite !(partialsubst_partialsubst x),
+             !(partialsubst_partialsubst x'); auto;
+     repeat (rewrite term_subst_notin by (cbn; varsdec));
+     cbn;
+     rewrite ?Vars.singleton_spec;
+     try apply IsSimple_partialsubst;
+     try apply noninter_issimple; cbn; try varsdec.
+
+     apply IH; auto;
+     rewrite !allvars_partialsubst; cbn; varsdec.
+Qed.
+
+Lemma AEq_trans f1 f2 f3 :
+ AlphaEq f1 f2 -> AlphaEq f2 f3 -> AlphaEq f1 f3.
+Proof.
+ revert f2 f3.
+ induction f1 as [h IH f1 LT] using form_height_ind.
+ destruct f1, f2, f3; cbn in *; simpl_height;
+  inversion_clear 1; inversion_clear 1; eauto.
+ set (vars :=
+        vars_unions [ (allvars f1); (allvars f2); (allvars f3) ]).
+ destruct (get_fresh_var vars) as (z1,Hz1). simpl_fresh vars Hz1.
+ apply AEq_rename_any with (z':=z1) in H1; [ |varsdec|varsdec].
+ apply AEq_rename_any with (z':=z1) in H3; [ |varsdec|varsdec].
+ apply AEqQu with z1; eauto. varsdec.
+Qed.
+
+Instance AEq_equiv : Equivalence AlphaEq.
+Proof.
+ split; [exact AEq_refl| exact AEq_sym | exact AEq_trans].
+Qed.
+
+Lemma AEq_partialsubst f f' :
+ AlphaEq f f' ->
+ forall x t,
+ IsSimple x t f -> IsSimple x t f' ->
+ AlphaEq (partialsubst x t f) (partialsubst x t f').
+Proof.
+ revert f'.
+ induction f as [h IH f LT] using form_height_ind.
+ destruct f, f'; intros EQ x t IS1 IS2; inversion_clear EQ;
+  cbn in *; simpl_height; auto.
+ - constructor; intuition.
+ - rename v0 into v'.
+   rename H0 into EQ.
+   clear q; rename q0 into q.
+   assert (IsSimple v (Var z) f)
+     by (apply noninter_issimple; cbn; varsdec).
+   assert (IsSimple v' (Var z) f')
+     by (apply noninter_issimple; cbn; varsdec).
+   repeat (case eqbspec; cbn); intros; auto.
+   + subst v; subst v'.
+     apply AEqQu with z; auto.
+   + subst v. clear IS1.
+     destruct IS2 as [->|(NI,IS2)]; [easy|].
+     rewrite vars_mem_false by trivial.
+     assert (~Vars.In x (freevars f')).
+     { case (eqbspec x z).
+       - intros ->; rewrite freevars_allvars; varsdec.
+       - intros NE.
+         apply AEq_freevars in EQ.
+         rewrite (freevars_partialsubst_subset' v' (Var z)); auto.
+         rewrite <- EQ.
+         rewrite freevars_partialsubst_subset; auto.
+         cbn. clear EQ H. varsdec. }
+     rewrite partialsubst_notin; auto.
+     apply AEqQu with z; auto.
+   + subst v'. clear IS2.
+     destruct IS1 as [->|(NI,IS1)]; [easy|].
+     rewrite vars_mem_false by trivial.
+     assert (~Vars.In x (freevars f)).
+     { case (eqbspec x z).
+       - intros ->; rewrite freevars_allvars; varsdec.
+       - intros NE.
+         apply AEq_freevars in EQ.
+         rewrite (freevars_partialsubst_subset' v (Var z)); auto.
+         rewrite EQ.
+         rewrite freevars_partialsubst_subset; auto.
+         cbn. clear EQ H. varsdec. }
+     rewrite partialsubst_notin; auto.
+     apply AEqQu with z; auto.
+   + destruct IS1 as [->|(NI1,IS1)]; [easy|].
+     destruct IS2 as [->|(NI2,IS2)]; [easy|].
+     rewrite !vars_mem_false by trivial.
+     set (vars :=
+            Vars.add x (Vars.add v (Vars.add v'
+              (vars_unions
+                 [ term_vars t; allvars f; allvars f'])))).
+     destruct (get_fresh_var vars) as (z',Hz').
+     simpl_fresh vars Hz'.
+     apply AEq_rename_any with (z' := z') in EQ;
+       [ |varsdec|varsdec].
+     clear z H H0 H1.
+     apply AEqQu with z';
+       [rewrite 2 allvars_partialsubst; varsdec|].
+     rewrite 2 (partialsubst_partialsubst x); auto;
+     try (rewrite !term_subst_notin by varsdec);
+     try (apply IH; auto); cbn; try varsdec;
+     try apply IsSimple_partialsubst; auto;
+     apply noninter_issimple; cbn; varsdec.
+Qed.
+
+Lemma AEq_SimpleSubst f1 f2 f1' f2' x t :
+ AlphaEq f1 f2 ->
+ SimpleSubst x t f1 f1' -> SimpleSubst x t f2 f2' ->
+ AlphaEq f1' f2'.
+Proof.
+ intros EQ S1 S2. rewrite SimpleSubst_carac in *.
+ destruct S1 as (<-,IS1).
+ destruct S2 as (<-,IS2).
+ apply AEq_partialsubst; auto.
+Qed.
+
+Lemma AEqQu_nosubst f f' q v :
+ AlphaEq f f' -> AlphaEq (Quant q v f) (Quant q v f').
+Proof.
+ intros.
+ set (vars := Vars.union (allvars f) (allvars f')).
+ destruct (get_fresh_var vars) as (z,Hz).
+ apply AEqQu with z. exact Hz. apply AEq_partialsubst; auto.
+ apply noninter_issimple. cbn. varsdec.
+ apply noninter_issimple. cbn. varsdec.
+Qed.
+
+Lemma AEqQu_rename0 f q v z :
+ IsSimple v (Var z) f -> ~Vars.In z (freevars f) ->
+ AlphaEq (Quant q v f) (Quant q z (partialsubst v (Var z) f)).
+Proof.
+ intros IS NI.
+ set (vars := Vars.add z (Vars.add v (allvars f))).
+ destruct (get_fresh_var vars) as (z',Hz').
+ apply AEqQu with z'.
+ - rewrite allvars_partialsubst. cbn. varsdec.
+ - case (eqbspec v z).
+   + intros ->.
+     rewrite (partialsubst_notin z (Var z)); auto. reflexivity.
+   + intros NE.
+     rewrite partialsubst_partialsubst; auto; try varsdec.
+     rewrite (partialsubst_notin z); auto.
+     cbn. rewrite eqb_refl. reflexivity.
+     cbn. varsdec.
+     apply noninter_issimple. cbn. varsdec.
+     cbn. rewrite eqb_refl.
+     apply IsSimple_partialsubst.
+     apply noninter_issimple. cbn. varsdec.
+Qed.
+
+(** Same, with weaker but clearer precondition *)
+
+Lemma AEqQu_rename f q v z :
+ ~Vars.In z (allvars f) ->
+ AlphaEq (Quant q v f) (Quant q z (partialsubst v (Var z) f)).
+Proof.
+ intros NI. apply AEqQu_rename0.
+ - apply noninter_issimple. cbn. varsdec.
+ - rewrite freevars_allvars; varsdec.
+Qed.
+
+(** The full substitution, first as a relation *)
+
+Definition Subst x t f f' :=
+  exists f0, AlphaEq f f0 /\ SimpleSubst x t f0 f'.
+
+Lemma SimpleSubst_Subst x t f f' :
+  SimpleSubst x t f f' -> Subst x t f f'.
+Proof.
+ intros. now exists f.
+Qed.
+
+Lemma Subst_compat x t f1 f2 f1' f2' :
+ AlphaEq f1 f2 -> Subst x t f1 f1' -> Subst x t f2 f2' ->
+  AlphaEq f1' f2'.
+Proof.
+ intros EQ (f1b & EQ1 & S1) (f2b & EQ2 & S2).
+ apply (AEq_SimpleSubst f1b f2b f1' f2' x t); auto.
+ transitivity f1. now symmetry.
+ transitivity f2; auto.
+Qed.
+
+(* Pseudo constructors for Subst. *)
+
+Lemma Subst_True x t : Subst x t True True.
+Proof.
+ now apply SimpleSubst_Subst.
+Qed.
+
+Lemma Subst_False x t : Subst x t False False.
+Proof.
+ now apply SimpleSubst_Subst.
+Qed.
+
+Lemma Subst_Pred x t p l :
+  Subst x t (Pred p l) (partialsubst x t (Pred p l)).
+Proof.
+ apply SimpleSubst_Subst. now apply SimpleSubst_partialsubst.
+Qed.
+
+Lemma Subst_Not x t f f' :
+  Subst x t f f' -> Subst x t (~f) (~f').
+Proof.
+  intros (f0 & EQ & SI). exists (~ f0)%form; auto.
+Qed.
+
+Lemma Subst_Op x t o f1 f2 f1' f2' :
+  Subst x t f1 f1' -> Subst x t f2 f2' ->
+  Subst x t (Op o f1 f2) (Op o f1' f2').
+Proof.
+  intros (f1b & EQ1 & SI1) (f2b & EQ2 & SI2).
+  exists (Op o f1b f2b); auto.
+Qed.
+
+Lemma Subst_Qu1 x t q f :
+  Subst x t (Quant q x f) (Quant q x f).
+Proof.
+  exists (Quant q x f). split; auto. reflexivity.
+Qed.
+
+Lemma Subst_Qu2 x t q v f f' :
+  x <> v ->
+  ~Vars.In v (term_vars t) ->
+  Subst x t f f' ->
+  Subst x t (Quant q v f) (Quant q v f').
+Proof.
+  intros NE NI (f0 & EQ & IS).
+  exists (Quant q v f0). auto using AEqQu_nosubst.
+Qed.
+
+Lemma Subst_Qu3 x t q v z f f' g :
+  x <> v ->
+  ~Vars.In z (freevars f) ->
+  Subst v (Var z) f f' ->
+  Subst x t (Quant q z f') (Quant q z g) ->
+  Subst x t (Quant q v f) (Quant q z g).
+Proof.
+  intros NE NI (f0 & EQ & SI) (h & EQ' & SI').
+  exists h. split; auto.
+  transitivity (Quant q z f'); auto.
+  transitivity (Quant q v f0).
+  apply AEqQu_nosubst; auto.
+  rewrite SimpleSubst_carac in SI. destruct SI as (<-,IS).
+  apply AEqQu_rename0; auto.
+  apply AEq_freevars in EQ. now rewrite <- EQ.
+Qed.
+
+Lemma Subst_subst x t f : Subst x t f (form_subst x t f).
+Proof.
+ unfold form_subst.
+ set (h := S (form_height f)).
+ assert (LT : form_height f < h) by (cbn; auto with * ).
+ clearbody h. revert x t f LT.
+ induction h as [|h IH]; [inversion 1|];
+  intros x t [ ] LT; cbn -[fresh_var] in *; simpl_height.
+ - apply Subst_True.
+ - apply Subst_False.
+ - apply Subst_Pred.
+ - apply Subst_Not; auto.
+ - apply Subst_Op; auto.
+ - set (vars := Vars.union _ _).
+   assert (Hz := fresh_var_ok vars).
+   set (z := fresh_var _) in *. clearbody z.
+   case eqbspec.
+   + intros ->. apply Subst_Qu1.
+   + intros NE.
+     destruct (Vars.mem v (term_vars t)) eqn:IN; cbn - [fresh_var].
+     * clear IN.
+       apply Subst_Qu3 with (form_substH h v (Var z) f); auto.
+       { rewrite freevars_allvars. varsdec. }
+       { apply Subst_Qu2; auto; try varsdec.
+         apply IH. now rewrite form_substH_height. }
+     * apply Subst_Qu2; auto.
+       rewrite <- Vars.mem_spec. now rewrite IN.
+Qed.
+
+Lemma Subst_exists x t f : exists f', Subst x t f f'.
+Proof.
+ exists (form_subst x t f). apply Subst_subst.
+Qed.
+
+
+(** Alpha equivalence, now as a boolean function *)
+
+Fixpoint alpha_equivH h f1 f2 :=
+  match h with
+  | 0 => false
+  | S h =>
+    match f1, f2 with
+    | True, True | False, False => true
+    | Pred p1 args1, Pred p2 args2 =>
+      (p1 =? p2) &&& (args1 =? args2)
+    | Not f1, Not f2 => alpha_equivH h f1 f2
+    | Op o1 f1 f1', Op o2 f2 f2' =>
+      (o1 =? o2) &&&
+      alpha_equivH h f1 f2 &&&
+      alpha_equivH h f1' f2'
+    | Quant q1 v1 f1', Quant q2 v2 f2' =>
+      (q1 =? q2) &&&
+      (let z := fresh_var (Vars.union (allvars f1) (allvars f2))
+       in
+       alpha_equivH h (form_subst v1 (Var z) f1') (form_subst v2 (Var z) f2'))
+    | _,_ => false
+    end
+  end.
+
+Definition alpha_equiv f1 f2 :=
+ alpha_equivH (S (Nat.max (form_height f1) (form_height f2))) f1 f2.
+
+Lemma alpha_equiv_ok f f' :
+  alpha_equiv f f' = true <-> AlphaEq f f'.
+Proof.
+ unfold alpha_equiv.
+ set (h := S _).
+ assert (LT : form_height f < h) by (unfold h; auto with *).
+ assert (LT' : form_height f' < h) by (unfold h; auto with *).
+ clearbody h. revert f f' LT LT'.
+ induction h as [|h IH]; [inversion 1|].
+ destruct f, f'; simpl; intros LT LT'; simpl_height; try easy.
+ - rewrite lazy_andb_iff, !eqb_eq.
+   split.
+   + now intros (<-,<-).
+   + now inversion_clear 1.
+ - rewrite IH by auto. split; auto. inversion_clear 1; auto.
+ - rewrite !lazy_andb_iff, !eqb_eq, 2 IH by auto.
+   split.
+   + intros ((<-,?),?); auto.
+   + now inversion_clear 1.
+ - set (vars := Vars.union _ _).
+   assert (Hz := fresh_var_ok vars).
+   set (z := fresh_var vars) in *. clearbody z.
+   rewrite <- 2 partialsubst_subst by
+    (auto; apply noninter_issimple; cbn; varsdec).
+   rewrite !lazy_andb_iff, !eqb_eq, IH by auto.
+   split.
+   + intros (<-,?). apply AEqQu with z; auto with set.
+   + inversion_clear 1. split; trivial.
+     apply AEq_rename_any with z0; auto. varsdec.
+Qed.
